full correctness of extended binary eucledian for Montgomery numbers

examples/modular_inversion/proofs/gcd.ec
@@ -3,14 +3,6 @@ require import AllCore.
 require import IntDiv Int.
 require import Gcd_props.
 
-op div_by2s (i : int) : int.
-axiom div_by2s1 u : 0 < u = 0 < (div_by2s u).
-axiom div_by2s2 u v : odd v => gcd (div_by2s u) v = gcd u v.
-axiom div_by2s3 u : odd (div_by2s u).
-axiom div_by2s4 u : 0 < u => even u =>  (div_by2s u) < u.
-axiom div_by2s5 u : u < 0 => even u =>  u < (div_by2s u).
-axiom div_by2s6 u : even u =>  div_by2s (u %/ 2) = div_by2s u.
-axiom div_by2s7 u : odd u =>  div_by2s u = u.
 
 
 module GCDAlgs = {
@@ -22,56 +14,12 @@ module GCDAlgs = {
       return t;
   }
 
-  proc main1(u : int, v : int) = {
-    var k, t;
-    (k,t) <- (0,0);
-    k <- 0;
-    while (even(u) /\ even(v)) {
-       k <- k + 1;
-       u <- u %/ 2;
-       v <- v %/ 2;
-    }
-    t <- if (odd u) then (-v) else u;
-    t <- div_by2s t; 
-    (u,v) <- if 0 < t then (t,v) else (u,-t);
-    t <- u - v;
+  proc main3(u : int, v : int) = {
+    var t <- 0;
+    t <- -v;
     while (t <> 0){     
       t <- div_by2s t;
       (u,v) <- if 0 < t then (t,v) else (u,-t);
-      t <- u - v;
-    }
-    return u*2^k;
-  }
-
-
-  proc main2(u : int, v : int) = {
-    var k, t;
-    (k,t) <- (0,0);    
-    k <- 0;
-    while (even(u) /\ even(v)) {
-       k <- k + 1;
-       u <- u %/ 2;
-       v <- v %/ 2;
-    }
-    t <- if (odd u) then (-v) else u;
-    t <- div_by2s t; 
-    (u,v) <- if 0 < t then (t,v) else (u,-t);
-    t <- u - v;    
-    while (t <> 0){     
-      t <- div_by2s t;
-      (u,v) <- if v < u then (t,v) else (u,-t);
-      t <- u - v;
-    }
-    return u*2^k;
-  }
-
-  proc main3(u : int, v : int) = {
-    var t <- 0;
-    (u,v) <- (u, div_by2s v);
-    t <- u - v;
-    while (t <> 0){     
-      t <- div_by2s t;
-      (u,v) <- if v < u then (t,v) else (u,-t);
       t <- u - v;
     }
     return u;
@@ -80,17 +28,15 @@ module GCDAlgs = {
 
   proc main4(u : int, v : int) = {
     var t <- 0;
-    v <@ simplify_t(v);
-    t <- u - v;
+    t <- -v;
     while (t <> 0){     
       t <@ simplify_t(t);
-      (u,v) <- if v < u then (t,v) else (u,-t);
+      (u,v) <- if 0 < t then (t,v) else (u,-t);
       t <- u - v;
     }
     return u;
   }
-
-
+  
   
 }.
     
@@ -113,21 +59,10 @@ skip. progress. smt. smt.
 qed.    
 
 
-lemma main3_main4 u_in v_in : equiv [ GCDAlgs.main3 ~ GCDAlgs.main4 : arg{1} = (u_in, v_in) /\ 0 < u_in /\ 0 < v_in
- /\ odd u_in /\ ={arg} ==> ={res} ].
-proc.
-seq 3 3 : (={t,u,v}).
-wp.
-ecall {2} (simplify_divby2s v{2}). wp.
-skip. progress. smt.
-while (={t,u,v}). wp.
-ecall {2} (simplify_divby2s t{2}). wp.
-skip. progress. skip. progress.
-qed.    
-
 
 lemma main3_term : phoare [GCDAlgs.main3 : odd u /\ 0 < u /\ 0 < v ==> true ] = 1%r.
-proc. sp.
+proc. unroll 3.
+rcondt 3. wp. skip. progress. smt()    .
 while (t = u - v /\ even t /\ odd u /\ odd v /\ 0 < u /\ 0 < v) (max u v).
 progress.    
 wp. skip. progress.
@@ -150,136 +85,11 @@ progress.
      have : u{hr} - v{hr} < x. smt.
     smt.
     smt.    
-    skip.
+wp.    skip.
 progress.
 smt.
-    smt. smt. smt.
+    smt. smt. smt. smt. smt.
 qed.    
-
-
-    
-    
-lemma gcd_alg_eq : equiv [ GCDAlgs.main1 ~ GCDAlgs.main2  : ={arg} 
-  ==> ={res} ].
-proof. proc.
-sp.
-while (={u,v,k,t} /\ t{1} = u{1} - v{1}).
-wp. skip. progress;smt.
-wp. while (={u,v,k,t} ).
-wp. skip. progress.
-skip. progress.
-qed.
-
-
-lemma gcd_alg u_in v_in : hoare [ GCDAlgs.main1 : arg = (u_in, v_in) /\ 0 < u_in /\ 0 < v_in 
-  ==> res = gcd u_in v_in ].
-proof.
-proc.
-seq 3 : (gcd u_in v_in = 2^k  * gcd u v /\ (odd u \/ odd v) /\ 0 < u /\ 0 < v /\ 0 <= k).
-sp.
-while (gcd u_in v_in = 2^k  * gcd u v /\ 0 < u /\ 0 < v /\ 0 <= k).
-wp.
-skip. progress.
-rewrite H.
-rewrite gcd1. auto. auto.
-have ->: 2 ^ (k{hr} + 1) = 2 ^ k{hr} * 2. smt.
-smt(@Int).
-smt(@Int). smt(@Int).
-smt(). skip. progress. smt(@Int). smt().
-seq 1 : (gcd u_in v_in = 2^k  * gcd t (if 0 < t then v else u) /\ (odd u \/ odd v)
- /\ t = (if odd u then -v else u) /\ 0 < u /\ 0 < v).
-wp. skip. progress.
-case (odd u{hr}).
-have -> : 0 < -v{hr} = false. smt. simplify.
-rewrite H.
-progress. congr.
-smt.                            (* prop of gcd *)
-progress. rewrite H. congr. rewrite H1. simplify. auto.
-seq 1 : ((if odd u then div_by2s (-v) else div_by2s u) = t /\ gcd u_in v_in = 2^k  * gcd t (if 0 < t then v else u) /\ (odd u \/ odd v)
- /\  odd t /\ (0 < t = !odd u) /\ 0 < u /\ 0 < v ).
-wp. skip. progress.
-smt().
-rewrite H.
-congr.
-case (odd u{hr}).
-have ->: 0 < -v{hr}  = false. smt(). simplify.
-have ->: 0 < div_by2s (-v{hr}) = false. smt(div_by2s1).  simplify.
-move => q.
-rewrite div_by2s2. auto. 
-smt.
-progress.
-rewrite H1. simplify.
-have ->: 0 < div_by2s (u{hr}) = true. smt(div_by2s1). simplify. smt.
-apply div_by2s3.
-case (odd u{hr}). simplify.
-smt.
-smt.
-seq 1 : (gcd u_in v_in = 2^k  * gcd t (if 0 < t then v else u) /\ odd t /\ odd u /\ odd v /\ (u = if 0 < t then t else u) /\ (v = if 0 < t then v else -t) /\ 0 < u /\ 0 < v ).
-wp.
-skip.
-progress.
-rewrite H.
-congr.
-smt().
-case (0 < t{hr}). smt().
-progress.
-rewrite  H2.
-case (odd u{hr}). simplify. auto.
-simplify. smt.
-rewrite H2.
-case (odd u{hr}). simplify. auto.
-smt.  simplify. smt.
-smt().
-smt().
-smt.
-smt.
-seq 1 : ((gcd u_in v_in = 2^k  * gcd t (if 0 < t then v else u) /\ even t /\ odd u /\ odd v)  /\  0 < u /\ 0 < v).
-wp. skip. progress.
-rewrite H. congr.
-case (0 < t{hr}).
-rewrite H3 H4.
-progress. rewrite H7. simplify.
-case (0 < t{hr} - v{hr}).
-progress. apply gcd6.
-progress. smt.
-rewrite H4.
-progress.
-rewrite H7. simplify.
-  case (0 < u{hr} + t{hr}).
-progress.
-smt.
-smt.
-smt(odd_even).
-while (gcd u_in v_in = 2^k  * gcd t (if 0 < t then v else u) /\ even t /\ odd u /\ odd v /\  0 <= u /\ 0 <= v).
-seq 1 : (gcd u_in v_in = 2^k  * gcd t (if 0 < t then v else u) /\ odd t /\ odd u /\ odd v /\ t <> 0 /\ 0 <= u /\ 0 <= v).
-wp. skip. progress. rewrite H. congr.
-smt.
-smt.
-smt.
-seq 1 : (gcd u_in v_in = 2^k  * gcd t (if 0 < t then v else u) /\ odd t /\ odd u /\ odd v /\ t <> 0 /\ (u = if 0 < t then t else u) /\ (v = if 0 < t then v else -t) /\ 0 <= u /\ 0 <= v) .
-wp. skip. progress.
-rewrite H. congr.
-case (0 < t{hr}). auto.
-auto.
-smt(). smt.
-smt().
-smt().
-smt.
-smt.
-wp. skip. progress.
-rewrite H. congr.
-case (0 < t{hr}). auto.
-rewrite H4.
-progress. rewrite H8. simplify.
-rewrite gcd6. smt.
-rewrite H5.
-progress. rewrite H8. simplify. smt.
-smt.
-skip. progress.
-smt.
-smt.
-smt.
-qed.
 
 
 
@@ -287,12 +97,15 @@ lemma gcd_odd_alg u_in v_in : hoare [ GCDAlgs.main3 : arg = (u_in, v_in) /\ 0 < 
  /\ odd u ==> res = gcd u_in v_in ].
 proof.
 proc.
-seq 2 : (gcd u_in v_in = gcd u v /\ odd u /\ odd v
+unroll 3. rcondt 3. wp. skip. smt.
+
+seq 4 : (gcd u_in v_in = gcd u v /\ odd u /\ odd v
   /\ 0 < u /\ 0 < v ).
 wp. skip. progress.
-smt.                            (* prop of gcd *)
+have ->: 0 < div_by2s (-v{hr}) = false. smt(div_by2s1). simplify.
+smt.                            
 smt.
-smt.
+smt. smt. smt.
 seq 1 : ((gcd u_in v_in = gcd t (if 0 < t then v else u) /\ even t /\ odd u /\ odd v)  /\  0 < u /\ 0 < v /\ t = u - v).
 wp. skip. progress.
 rewrite H. 
@@ -333,6 +146,20 @@ apply gcd_odd_alg.
 qed.    
 
 
+lemma main3_main4 u_in v_in : equiv [ GCDAlgs.main3 ~ GCDAlgs.main4 : arg{1} = (u_in, v_in) /\ 0 < u_in /\ 0 < v_in
+ /\ odd u_in /\ ={arg} ==> ={res} ].
+proc.
+seq 2 2 : (={t,u,v}).
+wp. skip. progress.
+(* ecall {2} (simplify_divby2s v{2}). wp. *)
+(* skip. progress. smt. *)
+while (={t,u,v}). wp.
+ecall {2} (simplify_divby2s t{2}). wp.
+skip. progress. skip. progress.
+qed.    
+
+
+
 lemma main4_correct_and_terminating u_in v_in : phoare [ GCDAlgs.main4 : arg = (u_in, v_in) /\ 0 < u_in /\ 0 < v_in /\ odd u ==> res = gcd u_in v_in ] = 1%r.
 bypr.
 progress.
@@ -342,4 +169,3 @@ progress.
 byequiv. symmetry.
 conseq (main3_main4 u_in v_in). smt(). smt(). auto. auto.
 qed.    
-
