examples/modular_inversion/proofs/gcd_props.ec
@@ -17,3 +17,13 @@ lemma gcd6 t v : gcd t v = gcd (t - v) v. smt. qed.
 op inv : int -> int -> int.
   (* add proper conditions *)
 axiom inv_ax u v : (inv u v) * v %% u = 1. 
+
+
+op div_by2s (i : int) : int.
+axiom div_by2s1 u : 0 < u = 0 < (div_by2s u).
+axiom div_by2s2 u v : odd v => gcd (div_by2s u) v = gcd u v.
+axiom div_by2s3 u : odd (div_by2s u).
+axiom div_by2s4 u : 0 < u => even u =>  (div_by2s u) < u.
+axiom div_by2s5 u : u < 0 => even u =>  u < (div_by2s u).
+axiom div_by2s6 u : even u =>  div_by2s (u %/ 2) = div_by2s u.
+axiom div_by2s7 u : odd u =>  div_by2s u = u.
